tests/lean/run/1954.lean
@@ -1,2 +1,2 @@
-def all (p : ℕ → Prop) : Prop := ∀x, p x
-example {p : ℕ → Prop} (h : all p) : p 0 := h 0
+def all (p : Nat → Prop) : Prop := ∀x, p x
+example {p : Nat → Prop} (h : all p) : p 0 := h 0
