tests/lean/include_out_param.lean
@@ -1,9 +1,0 @@
-class c (α : Type) (β : outParam Type) :=
-(n : α → Nat)
-
-variables {α β : Type} [c α β]
-
-def f : Nat := 1
-#print f -- don't include anything
-def g (a : α) : Nat := c.n a
-#print g -- include everything
