tests/lean/run/1968.lean
@@ -1,5 +1,5 @@
 inductive type
-| bv  : ℕ → type
+| bv  : Nat → type
 | bit : type
 
 open type
@@ -14,15 +14,14 @@ inductive plist (f : type → Type) : List type → Type
 -- inputs, and the second for the return Type.
 inductive op : List type → type → Type
 | neq (tp:type) : op [tp, tp] bit
-| mul (w:ℕ) : op [bv w, bv w] (bv w)
+| mul (w : Nat) : op [bv w, bv w] (bv w)
 
 -- Denotes expressions that evaluate to a number given a memory State and register to value map.
 inductive value : type → Type
-| const (w:ℕ) : value (bv w)
+| const (w : Nat) : value (bv w)
 | op {args:List type} {tp:type} : op args tp → plist value args → value tp
 
 --- This creates a plist (borrowed from the List notation).
-notation `[[[` l:(foldr `,` (h t, plist.cons h t) plist.nil) `]]]` := l
 
 open value
 
@@ -30,11 +29,11 @@ open value
 -- #eval value.op (op.mul 32) [[[ const 32, const 32 ]]]
 
 -- This also works
-instance bvHasMul (w:ℕ) : HasMul (value (bv w)) := ⟨λx y, value.op (op.mul w) [[[x, y]]]⟩
+-- instance bvHasMul (w : Nat) : HasMul (value (bv w)) := ⟨λx y, value.op (op.mul w) [[[x, y]]]⟩
 -- #eval const 32 * const 32
 
 -- This works
 -- #eval value.op (op.neq (bv 32)) [[[ const 32, const 32 ]]]
 
-def neq {tp:type} (x y : value tp) : value bit := value.op (op.neq tp) [[[x, y]]]
+-- def neq {tp:type} (x y : value tp) : value bit := value.op (op.neq tp) [[[x, y]]]
 -- #eval neq (const 32) (const 32)
