tests/lean/run/float_cases_bug.lean
@@ -1,2 +1,2 @@
 def foo (xs : List Nat) :=
-xs.span (λ n, ↑(decide (n = 1)))
+xs.span (λ n, coe (decide (n = 1)))
